a)
|  1 2 3  1 |   | 1 2  3  1 |   | 1  2  3  1 |
|  0 4 0  2 | = | 0 4  0  2 | = | 0  4  0  2 | = (-1) * 1 *
| -3 1 1 -1 |   | 0 7 10  2 |   | 0 -1 10 -2 |
|  4 1 5 -2 |   | 1 2  6 -3 |   | 0  0  3 -2 |

b)
| 1  1  1 2 |
| 2 -1  1 3 | = (-1)^4 * | M13 | + (-1)^5 * | M23 | + (-1)^6 * | M33 | + (-1)^7 * | M43 |
| 1  2 -1 2 |
| 3  3  2 1 |
=

vd2.
r(A) = 3
=>
      |  1 2 0 |
|A| = |  1 1 m | != 0 <=> |A| = 1 -2m - 2 != 0 <=> m != -1/2
      | -1 0 1 |

vd1.
    | 1  1  1  1 |        | 1 1  1 1 |        | 1 1  1 1 |        | 1 2  1 1 |
A = | 1  3 -2  4 | => A = | 0 2 -3 3 | => A = | 0 3 -3 2 | => A = | 0 0 -3 2 |
    | 1 -1  4 -2 |        | 0 4 -6 6 |        | 0 0  0 0 |        | 0 0  0 0 |
=> r(A) = 2

vd2.
    | 1 1 -3 |    | 1   1  -3 |    | 1  1     -3 |
A = | 2 1  m | => | 0  -1 m+6 | => | 0 -1    m+6 |
    | 1 m  3 |    | 0 m-1   6 |    | 0  0 m^2+5m |

TH1: m^2+5m = 0 => m = -5 hay m = 0 => r(A) = 2
TH2: m^2+5m != 0 => m != -5 va m != 0 => r(A) = 3

    | 1 2 3 |
A = | 2 5 3 | => |A| = 40 + 0 + 6 - 15 - 32 - 0 = -1
    | 1 0 8 |

                |  40 -13 -5 |    | -40 13  5 |
A^(-1) = -1/1 * | -16   5  2 | => |  16 -5 -2 |
                |  -9   3  1 |    |   9 -3 -1 |

    [ 1 2 3 | 1 0 0 ]    [ 1  2  3 |  1  0 0 ] 
A = | 2 5 3 | 0 1 0 | => | 0  1 -3 | -2 -1 0 |
    [ 1 0 8 | 0 0 1 ]    [ 0 -2  5 | -1  0 1 ]
   [ 1 0 -3 |
=> | 0 1 -3 | 
   [ 0 0 -1 |
    | 1 2 3 |    | 1  2  3 |    | 1 2   3 |
A = | 2 5 3 | => | 0  1 -3 | => | 0 1  -3 |
    | 1 0 8 |    | 0 -2  5 |    | 0 0 -11 |

A^(-1) = | 1 2